Fix `bvi_let`

compiler/backend/bvi_letScript.sml
@@ -90,7 +90,10 @@ Definition compile_def:
      [Raise (HD (compile env d [x1]))]) /\
   (compile env d [Op op xs] = [Op op (compile env d xs)]) /\
   (compile env d [Tick x] = [Tick (HD (compile env d [x]))]) /\
-  (compile env d [Force loc v] = [Force loc v]) /\
+  (compile env d [Force loc v] =
+     case LLOOKUP env v of
+     | SOME n => [Force loc (v + n)]
+     | _ => [Force loc (v + d)]) /\
   (compile env d [Call t dest xs h] =
      [Call t dest (compile env d xs)
          (case h of NONE => NONE
@@ -128,7 +131,10 @@ Definition compile_sing_def:
      (Raise ((compile_sing env d x1)))) /\
   (compile_sing env d (Op op xs) = (Op op (compile_list env d xs))) /\
   (compile_sing env d (Tick x) = (Tick (compile_sing env d x))) /\
-  (compile_sing env d (Force loc v) = (Force loc v)) /\
+  (compile_sing env d (Force loc v) =
+     case LLOOKUP env v of
+     | SOME n => Force loc (v + n)
+     | _ => Force loc (v + d)) /\
   (compile_sing env d (Call t dest xs h) =
      (Call t dest (compile_list env d xs)
          (case h of NONE => NONE
